changed the beepl compiler to produce ok/error

cfrontend/BeePL_Csyntax.v
@@ -1,19 +1,24 @@
 Require Import String ZArith Coq.FSets.FMapAVL Coq.Structures.OrderedTypeEx Coq.Strings.BinaryString.
 Require Import Coq.FSets.FSetProperties Coq.FSets.FMapFacts FMaps FSetAVL Nat PeanoNat Coq.Lists.List.
-Require Import Coq.Arith.EqNat Coq.ZArith.Int Integers AST Maps Ctypes.
-Require Import BeePL_aux BeePL Csyntax.
+Require Import Coq.Arith.EqNat Coq.ZArith.Int Integers AST Maps Ctypes Coqlib.
+Require Import BeePL_aux BeePL Csyntax Errors.
 
+Local Open Scope string_scope.
+Local Open Scope error_monad_scope.
 
 (****** Translation from BeePL to Csyntax ******)
 
 Section translate_types.
 
-Variable transBeePL_type : BeeTypes.type -> Ctypes.type.
+Variable transBeePL_type : BeeTypes.type -> res Ctypes.type.
 
-Fixpoint transBeePL_types (ts : list BeeTypes.type) : Ctypes.typelist :=
+(* Translates a list of BeePL types to list of Clight types *) 
+Fixpoint transBeePL_types (ts : list BeeTypes.type) : res Ctypes.typelist :=
 match ts with 
-| nil => Tnil
-| t :: ts => Tcons (transBeePL_type t) (transBeePL_types ts)
+| nil => OK Tnil
+| t :: ts => do ct <- (transBeePL_type t);
+             do cts <- (transBeePL_types ts);
+             OK (Tcons ct cts)
 end.
 
 End translate_types.
@@ -45,25 +50,25 @@ match i with
 end.
 
 (* Translation of BeePL types to Clight Types *) 
-Fixpoint transBeePL_type (t : BeeTypes.type) : Ctypes.type :=
+Fixpoint transBeePL_type (t : BeeTypes.type) : res Ctypes.type :=
 match t with 
-| BeeTypes.Ptype (BeeTypes.Tunit) => (Tint I8 Unsigned {| attr_volatile := false; attr_alignas := Some 1%N |}) (* Fix me *)
-| BeeTypes.Ptype (BeeTypes.Tint sz s) => (Tint (transBeePL_isize_cisize sz) (transBeePL_sign_csign s)
-                                          {| attr_volatile := false; attr_alignas := Some (compute_align sz) |})
-| BeeTypes.Ptype (BeeTypes.Tbool) => (Tint I8 Unsigned {| attr_volatile := false; attr_alignas := Some 1%N |}) 
+| BeeTypes.Ptype (BeeTypes.Tunit) => OK (Tint I8 Unsigned {| attr_volatile := false; attr_alignas := Some 1%N |}) (* Fix me *)
+| BeeTypes.Ptype (BeeTypes.Tint sz s) => OK (Tint (transBeePL_isize_cisize sz) (transBeePL_sign_csign s)
+                                              {| attr_volatile := false; attr_alignas := Some (compute_align sz) |})
+| BeeTypes.Ptype (BeeTypes.Tbool) => OK (Tint I8 Unsigned {| attr_volatile := false; attr_alignas := Some 1%N |}) 
 | BeeTypes.Reftype h b => match b with 
-                          | BeeTypes.Bprim (BeeTypes.Tunit) => Tpointer Tvoid {| attr_volatile := false; attr_alignas := Some 1%N |}
-                          | BeeTypes.Bprim (BeeTypes.Tint sz s) => Tpointer (Tint (transBeePL_isize_cisize sz) (transBeePL_sign_csign s)
+                          | BeeTypes.Bprim (BeeTypes.Tunit) => OK (Tpointer Tvoid {| attr_volatile := false; attr_alignas := Some 1%N |})
+                          | BeeTypes.Bprim (BeeTypes.Tint sz s) => OK (Tpointer (Tint (transBeePL_isize_cisize sz) (transBeePL_sign_csign s)
                                                                              {| attr_volatile := false; attr_alignas := Some (compute_align sz) |})
-                                                              {| attr_volatile := false; attr_alignas := Some 8%N |}
-                          | BeeTypes.Bprim (BeeTypes.Tbool) => Tpointer (Tint I8 Unsigned {| attr_volatile := false; 
+                                                              {| attr_volatile := false; attr_alignas := Some 8%N |})
+                          | BeeTypes.Bprim (BeeTypes.Tbool) => OK (Tpointer (Tint I8 Unsigned {| attr_volatile := false; 
                                                                                              attr_alignas := Some 1%N |}) 
-                                                               {| attr_volatile := false; attr_alignas := Some 8%N |}
+                                                                   {| attr_volatile := false; attr_alignas := Some 8%N |})
                           end
-| BeeTypes.Ftype ts ef t => Tfunction (transBeePL_types transBeePL_type ts) 
-                                        (transBeePL_type t)  
-                                        {| cc_vararg := Some (Z.of_nat(length(ts))); cc_unproto := false; cc_structret := false |}  
-end. 
+| BeeTypes.Ftype ts ef t => do ats <- (transBeePL_types transBeePL_type ts);
+                            do rt <- (transBeePL_type t);
+                            OK (Tfunction ats rt {| cc_vararg := Some (Z.of_nat(length(ts))); cc_unproto := false; cc_structret := false |})  
+end.
 
 Definition bool_to_int (b : bool) : int :=
 match b with 
@@ -71,6 +76,7 @@ match b with
 | false => (Int.repr 0)
 end.
 
+(* Translates BeePL values to C values *)
 Definition transBeePL_value_cvalue (v : BeePL_mem.value) : Values.val :=
 match v with 
 | BeePL_mem.Vunit => Values.Vint (Int.repr 0) (* Fix me *)
@@ -81,12 +87,15 @@ end.
 
 Section transBeePL_exprs.
 
-Variables transBeePL_expr_expr : BeePL.expr -> Csyntax.expr.
+Variables transBeePL_expr_expr : BeePL.expr -> res Csyntax.expr.
 
-Fixpoint transBeePL_expr_exprs (es : list BeePL.expr) : Csyntax.exprlist :=
+(* Translates list of BeePL expressions to list of C expressions *)
+Fixpoint transBeePL_expr_exprs (es : list BeePL.expr) : res Csyntax.exprlist :=
 match es with 
-| nil => Enil 
-| e :: es => Econs (transBeePL_expr_expr e) (transBeePL_expr_exprs es)
+| nil => OK Enil 
+| e :: es => do ce <- (transBeePL_expr_expr e);
+             do ces <- (transBeePL_expr_exprs es);
+             OK (Econs ce ces)
 end.
 
 End transBeePL_exprs.
@@ -123,51 +132,73 @@ match es with
 | Econs e1 es => (e1 :: exprlist_list_expr es)
 end.
 
-Fixpoint transBeePL_expr_expr (e : BeePL.expr) : Csyntax.expr := 
+Fixpoint transBeePL_expr_expr (e : BeePL.expr) : res Csyntax.expr := 
 match e with 
-| Var x => Evar x.(BeePL_mem.vname) (transBeePL_type (x.(BeePL_mem.vtype)))
+| Var x => do xt <- (transBeePL_type (x.(BeePL_mem.vtype)));
+           OK (Evar x.(BeePL_mem.vname) xt)
 | Const c t => match c with 
-               | ConsInt i => Eval (Values.Vint i) (transBeePL_type t)
-               | ConsBool b => Eval (Values.Vint (bool_to_int b)) (transBeePL_type t)
-               | ConsUnit => Eval (Values.Vint (Int.repr 0)) (transBeePL_type t)
+               | ConsInt i => do it <- (transBeePL_type t); OK (Eval (Values.Vint i) it)
+               | ConsBool b => do bt <- (transBeePL_type t); OK (Eval (Values.Vint (bool_to_int b)) bt)
+               | ConsUnit => do ut <- (transBeePL_type t); OK (Eval (Values.Vint (Int.repr 0)) ut) 
                end
-| App r e es t => Ecall (transBeePL_expr_expr e) (transBeePL_expr_exprs transBeePL_expr_expr es) (transBeePL_type t)  
+| App r e es t => do ce <- (transBeePL_expr_expr e); 
+                  do ces <- (transBeePL_expr_exprs transBeePL_expr_expr es);
+                  do ct <- (transBeePL_type t);
+                  OK (Ecall ce ces ct)
 | Prim b es t => match b with 
-                 | Ref => Eaddrof (hd (Eval (Values.Vint (Int.repr 0))
-                                      (Tint I32 Signed {| attr_volatile := false; attr_alignas := Some 4%N |}))
-                                  (exprlist_list_expr (transBeePL_expr_exprs transBeePL_expr_expr es))) 
-                          (transBeePL_type t)   
-                 | Deref => Ederef (hd  (Eval (Values.Vint (Int.repr 0))
+                 | Ref => do ces <- (transBeePL_expr_exprs transBeePL_expr_expr es);
+                          do ct <- (transBeePL_type t);
+                          OK (Eaddrof (hd (Eval (Values.Vint (Int.repr 0))
                                         (Tint I32 Signed {| attr_volatile := false; attr_alignas := Some 4%N |}))
-                                    (exprlist_list_expr (transBeePL_expr_exprs transBeePL_expr_expr es))) 
-                           (transBeePL_type t)   
-                 | Massgn => Eassign (hd  (Eval (Values.Vint (Int.repr 0))
+                                      (exprlist_list_expr ces)) 
+                              ct) 
+                 | Deref => do ces <- (transBeePL_expr_exprs transBeePL_expr_expr es);
+                            do ct <- (transBeePL_type t);
+                            OK (Ederef (hd  (Eval (Values.Vint (Int.repr 0))
+                                        (Tint I32 Signed {| attr_volatile := false; attr_alignas := Some 4%N |}))
+                                       (exprlist_list_expr ces)) 
+                                ct)   
+                 | Massgn => do ces <- (transBeePL_expr_exprs transBeePL_expr_expr es);
+                             do ct <- (transBeePL_type t);
+                             OK (Eassign (hd  (Eval (Values.Vint (Int.repr 0))
                                          (Tint I32 Signed {| attr_volatile := false; attr_alignas := Some 4%N |}))
-                                         (exprlist_list_expr (transBeePL_expr_exprs transBeePL_expr_expr es)))
+                                         (exprlist_list_expr ces))
                                     (hd  (Eval (Values.Vint (Int.repr 0))
                                        (Tint I32 Signed {| attr_volatile := false; attr_alignas := Some 4%N |}))
-                                 (tl (exprlist_list_expr (transBeePL_expr_exprs transBeePL_expr_expr es))))
-                             (transBeePL_type t)
-                 | Run h => Eval (Values.Vundef) Tvoid (* Fix me *)
-                 | Uop o => Eunop (transBeePL_uop_uop o) 
-                            (hd  (Eval (Values.Vint (Int.repr 0))
+                                     (tl (exprlist_list_expr ces)))
+                                 ct)
+                 | Run h => OK (Eval (Values.Vundef) Tvoid) (* Fix me *)
+                 | Uop o => do ces <- (transBeePL_expr_exprs transBeePL_expr_expr es);
+                            do ct <- (transBeePL_type t);
+                            OK (Eunop (transBeePL_uop_uop o) 
+                                (hd  (Eval (Values.Vint (Int.repr 0))
                                        (Tint I32 Signed {| attr_volatile := false; attr_alignas := Some 4%N |}))
-                                 (exprlist_list_expr (transBeePL_expr_exprs transBeePL_expr_expr es))) 
-                            (transBeePL_type t) 
-                 | Bop o => Ebinop (transBeePL_bop_bop o) 
-                            (hd  (Eval (Values.Vint (Int.repr 0))
+                                (exprlist_list_expr ces)) 
+                                ct)
+                 | Bop o => do ces <- (transBeePL_expr_exprs transBeePL_expr_expr es);
+                            do ct <- (transBeePL_type t);
+                            OK (Ebinop (transBeePL_bop_bop o) 
+                                  (hd  (Eval (Values.Vint (Int.repr 0))
                                        (Tint I32 Signed {| attr_volatile := false; attr_alignas := Some 4%N |}))
-                                 (exprlist_list_expr (transBeePL_expr_exprs transBeePL_expr_expr es))) 
-                            (hd  (Eval (Values.Vint (Int.repr 0))
+                                   (exprlist_list_expr ces)) 
+                                  (hd  (Eval (Values.Vint (Int.repr 0))
                                        (Tint I32 Signed {| attr_volatile := false; attr_alignas := Some 4%N |}))
-                                 (tl (exprlist_list_expr (transBeePL_expr_exprs transBeePL_expr_expr es))))
-                            (transBeePL_type t)
+                                    (tl (exprlist_list_expr ces)))
+                                ct)
                  end 
-| Bind x t e e' t' => Ecomma (Eassign (Evar x (transBeePL_type t)) (transBeePL_expr_expr e) (transBeePL_type t)) 
-                             (transBeePL_expr_expr e') (transBeePL_type t')
-| Cond e e' e'' t => Econdition (transBeePL_expr_expr e) (transBeePL_expr_expr e') (transBeePL_expr_expr e'') (transBeePL_type t)
-| Addr l => Eval (Values.Vptr l.(BeePL_mem.lname) (Ptrofs.of_ints (Int.repr 0))) (transBeePL_type l.(BeePL_mem.ltype))
-| Hexpr h e t => Eval (Values.Vundef) Tvoid (* FIX ME *)
+| Bind x t e e' t' => do ct <- (transBeePL_type t);
+                      do ce <- (transBeePL_expr_expr e);
+                      do ce' <- (transBeePL_expr_expr e');
+                      do ct' <- (transBeePL_type t');
+                      OK (Ecomma (Eassign (Evar x ct) ce ct) ce' ct') 
+| Cond e e' e'' t => do ce <- (transBeePL_expr_expr e);
+                     do ce' <- (transBeePL_expr_expr e');
+                     do ce'' <- (transBeePL_expr_expr e'');
+                     do ct <- (transBeePL_type t);
+                     OK (Econdition ce ce' ce'' ct)  
+| Addr l => do ct <- (transBeePL_type l.(BeePL_mem.ltype));
+            OK (Eval (Values.Vptr l.(BeePL_mem.lname) (Ptrofs.of_ints (Int.repr 0))) ct)
+| Hexpr h e t => OK (Eval (Values.Vundef) Tvoid) (* FIX ME *)
 end.
 
 Definition check_var_const (e : BeePL.expr) : bool :=
@@ -178,93 +209,117 @@ match e with
 end.
 
 
-Definition transBeePL_expr_st (e : BeePL.expr) : Csyntax.statement :=
+Definition transBeePL_expr_st (e : BeePL.expr) : res Csyntax.statement :=
 match e with 
-| Var x => Sreturn (Some (Evalof (Evar x.(BeePL_mem.vname) (transBeePL_type x.(BeePL_mem.vtype))) (transBeePL_type x.(BeePL_mem.vtype))))
-| Const c t => Sreturn (Some (Evalof (match c with 
-                                      | ConsInt i => Eval (Values.Vint i) (transBeePL_type t)
-                                      | ConsBool b => Eval (Values.Vint (bool_to_int b)) (transBeePL_type t)
-                                      | ConsUnit => Eval (Values.Vint (Int.repr 0)) (transBeePL_type t)
-                                      end) (transBeePL_type t)))
-| App r e es t => Sdo (Ecall (transBeePL_expr_expr e) (transBeePL_expr_exprs transBeePL_expr_expr es) (transBeePL_type t))  
+| Var x => do ct <- (transBeePL_type x.(BeePL_mem.vtype));
+           OK (Sreturn (Some (Evalof (Evar x.(BeePL_mem.vname) ct) ct)))
+| Const c t => do ct <- (transBeePL_type t);
+               OK (Sreturn (Some (Evalof (match c with 
+                                      | ConsInt i => Eval (Values.Vint i) ct
+                                      | ConsBool b => Eval (Values.Vint (bool_to_int b)) ct
+                                      | ConsUnit => Eval (Values.Vint (Int.repr 0)) ct
+                                      end) ct)))
+| App r e es t => do ce <- (transBeePL_expr_expr e);
+                  do ces <- (transBeePL_expr_exprs transBeePL_expr_expr es);
+                  do ct <- (transBeePL_type t);
+                  OK (Sdo (Ecall ce ces ct))  
 | Prim b es t => match b with 
-                 | Ref =>  Sdo (Eaddrof (hd  (Eval (Values.Vint (Int.repr 0))
+                 | Ref => do ces <- (transBeePL_expr_exprs transBeePL_expr_expr es);
+                          do ct <- (transBeePL_type t);
+                          OK (Sdo (Eaddrof (hd  (Eval (Values.Vint (Int.repr 0))
                                         (Tint I32 Signed {| attr_volatile := false; attr_alignas := Some 4%N |}))
-                                        (exprlist_list_expr (transBeePL_expr_exprs transBeePL_expr_expr es))) 
-                                (transBeePL_type t))   
-                 | Deref => Sdo (Ederef (hd  (Eval (Values.Vint (Int.repr 0))
+                                        (exprlist_list_expr ces)) 
+                                   ct))   
+                 | Deref => do ces <- (transBeePL_expr_exprs transBeePL_expr_expr es);
+                            do ct <- (transBeePL_type t);
+                            OK (Sdo (Ederef (hd  (Eval (Values.Vint (Int.repr 0))
                                         (Tint I32 Signed {| attr_volatile := false; attr_alignas := Some 4%N |}))
-                                         (exprlist_list_expr (transBeePL_expr_exprs transBeePL_expr_expr es))) 
-                                 (transBeePL_type t))   
-                 | Massgn => Sdo (Eassign (hd  (Eval (Values.Vint (Int.repr 0))
+                                         (exprlist_list_expr ces)) 
+                                     ct))   
+                 | Massgn => do ces <- (transBeePL_expr_exprs transBeePL_expr_expr es);
+                             do ct <- (transBeePL_type t);
+                             OK (Sdo (Eassign (hd  (Eval (Values.Vint (Int.repr 0))
                                                (Tint I32 Signed {| attr_volatile := false; attr_alignas := Some 4%N |}))
-                                               (exprlist_list_expr (transBeePL_expr_exprs transBeePL_expr_expr es)))
-                                          (hd  (Eval (Values.Vint (Int.repr 0))
+                                               (exprlist_list_expr ces))
+                                              (hd  (Eval (Values.Vint (Int.repr 0))
                                                (Tint I32 Signed {| attr_volatile := false; attr_alignas := Some 4%N |}))
-                                               (tl (exprlist_list_expr (transBeePL_expr_exprs transBeePL_expr_expr es))))
-                                 (transBeePL_type t)) 
-                 | Run h => Sdo (Eval (Values.Vundef) Tvoid) (* Fix me *)
-                 | Uop o => Sdo (Eunop (transBeePL_uop_uop o) 
-                                 (hd  (Eval (Values.Vint (Int.repr 0))
+                                               (tl (exprlist_list_expr ces)))
+                                      ct)) 
+                 | Run h => OK (Sdo (Eval (Values.Vundef) Tvoid)) (* Fix me *)
+                 | Uop o => do ces <- (transBeePL_expr_exprs transBeePL_expr_expr es);
+                            do ct <- (transBeePL_type t); 
+                            OK (Sdo (Eunop (transBeePL_uop_uop o) 
+                                     (hd (Eval (Values.Vint (Int.repr 0))
                                        (Tint I32 Signed {| attr_volatile := false; attr_alignas := Some 4%N |}))
-                                      (exprlist_list_expr (transBeePL_expr_exprs transBeePL_expr_expr es))) 
-                                 (transBeePL_type t)) 
-                 | Bop o => Sdo (Ebinop (transBeePL_bop_bop o) 
-                            (hd  (Eval (Values.Vint (Int.repr 0))
-                                       (Tint I32 Signed {| attr_volatile := false; attr_alignas := Some 4%N |}))
-                                 (exprlist_list_expr (transBeePL_expr_exprs transBeePL_expr_expr es))) 
-                            (hd  (Eval (Values.Vint (Int.repr 0))
-                                       (Tint I32 Signed {| attr_volatile := false; attr_alignas := Some 4%N |}))
-                                 (tl (exprlist_list_expr (transBeePL_expr_exprs transBeePL_expr_expr es))))
-                            (transBeePL_type t))
+                                      (exprlist_list_expr ces)) 
+                                     ct)) 
+                 | Bop o => do ces <- (transBeePL_expr_exprs transBeePL_expr_expr es);
+                            do ct <- (transBeePL_type t);
+                            OK (Sdo (Ebinop (transBeePL_bop_bop o) 
+                                     (hd (Eval (Values.Vint (Int.repr 0))
+                                         (Tint I32 Signed {| attr_volatile := false; attr_alignas := Some 4%N |}))
+                                        (exprlist_list_expr ces)) 
+                                     (hd (Eval (Values.Vint (Int.repr 0))
+                                         (Tint I32 Signed {| attr_volatile := false; attr_alignas := Some 4%N |}))
+                                      (tl (exprlist_list_expr ces)))
+                                     ct))
                  end 
 | Bind x t e e' t' => match e' with 
                       (* no side-effect case *)
-                      | Var x' => Ssequence (Sdo (Eassign (Evar x (transBeePL_type t)) 
-                                                            (transBeePL_expr_expr e) 
-                                                    Tvoid)) 
-                                               (Sreturn (Some (Evalof (transBeePL_expr_expr e') (transBeePL_type (BeePL.typeof_expr (e'))))))
-                      | Const c t => Ssequence (Sdo (Eassign (Evar x (transBeePL_type t)) (transBeePL_expr_expr e) Tvoid)) 
-                                               (Sreturn (Some (transBeePL_expr_expr e')))
+                      | Var x' => do ce <- (transBeePL_expr_expr e);
+                                  do ce' <- (transBeePL_expr_expr e'); 
+                                  do ct <- (transBeePL_type t);
+                                  do ct' <- (transBeePL_type t');
+                                  do rt <- (transBeePL_type (BeePL.typeof_expr (e')));
+                                  OK (Ssequence (Sdo (Eassign (Evar x ct) ce Tvoid))
+                                                (Sreturn (Some (Evalof ce' rt))))
+                      | Const c t => do ct <- (transBeePL_type t); 
+                                     do ce <- (transBeePL_expr_expr e);
+                                     do ce' <- (transBeePL_expr_expr e');
+                                     OK (Ssequence (Sdo (Eassign (Evar x ct) ce Tvoid)) 
+                                                   (Sreturn (Some ce')))
                       (* can produce side-effects *)
-                      | _ => Ssequence (Sdo (Eassign (Evar x (transBeePL_type t)) (transBeePL_expr_expr e) Tvoid)) 
-                                       (Sdo (transBeePL_expr_expr e'))
+                      | _ => do ct <- (transBeePL_type t);
+                             do ce <- (transBeePL_expr_expr e);
+                             do ce' <- (transBeePL_expr_expr e');
+                             OK (Ssequence (Sdo (Eassign (Evar x ct) ce Tvoid)) 
+                                           (Sdo ce'))
                     end
-| Cond e e' e'' t' => if (check_var_const e' && check_var_const e'') (* check for expressions with side-effects *)
-                      then Sifthenelse (transBeePL_expr_expr e) 
-                                       (Sreturn (Some (Evalof (transBeePL_expr_expr e') (transBeePL_type t')))) 
-                                       (Sreturn (Some (Evalof (transBeePL_expr_expr e'') (transBeePL_type t'))))
-                      else if (check_var_const e') then Sifthenelse (transBeePL_expr_expr e) 
-                                                        (Sreturn (Some (Evalof (transBeePL_expr_expr e')(transBeePL_type t')))) 
-                                                        (Sdo (transBeePL_expr_expr e''))
+| Cond e e' e'' t' => do ce <- (transBeePL_expr_expr e);
+                      do ce' <- (transBeePL_expr_expr e');
+                      do ce'' <- (transBeePL_expr_expr e'');
+                      do ct' <- (transBeePL_type t');
+                      if (check_var_const e' && check_var_const e'') (* check for expressions with side-effects *)
+                      then OK (Sifthenelse ce (Sreturn (Some (Evalof ce' ct'))) (Sreturn (Some (Evalof ce'' ct'))))
+                      else if (check_var_const e') then OK (Sifthenelse ce (Sreturn (Some (Evalof ce' ct'))) (Sdo ce''))
                                                    else if (check_var_const e'') 
-                                                        then Sifthenelse (transBeePL_expr_expr e) 
-                                                                         (Sdo (transBeePL_expr_expr e')) 
-                                                                         (Sreturn (Some (Evalof (transBeePL_expr_expr e'') 
-                                                                                                 (transBeePL_type t'))))
-                                                        else Sifthenelse (transBeePL_expr_expr e) 
-                                                                         (Sdo (transBeePL_expr_expr e'))
-                                                                         (Sdo (transBeePL_expr_expr e''))
+                                                        then OK (Sifthenelse ce (Sdo ce') (Sreturn (Some (Evalof ce'' ct'))))
+                                                        else OK (Sifthenelse ce (Sdo ce') (Sdo ce''))
                       
-| Addr l => Sdo (Eval (Values.Vptr l.(BeePL_mem.lname) (Ptrofs.of_ints (Int.repr 0))) (transBeePL_type l.(BeePL_mem.ltype)))
-| Hexpr h e t => Sdo (Eval (Values.Vundef) Tvoid) (* FIX ME *)
+| Addr l => do ct <- (transBeePL_type l.(BeePL_mem.ltype)); 
+            OK (Sdo (Eval (Values.Vptr l.(BeePL_mem.lname) (Ptrofs.of_ints (Int.repr 0))) ct))
+| Hexpr h e t => OK (Sdo (Eval (Values.Vundef) Tvoid)) (* FIX ME *)
 end.
 
 Definition default_cc (fd : fun_decl) : calling_convention := 
 {| cc_vararg := Some (Z.of_nat (length (fd.(args)))); cc_unproto := false; cc_structret := false |}.
 
-(* For now we have only internal functions: later change it to include both the case *)
-Definition BeePLfd_function (fd : fun_decl) : (Ctypes.fundef function) :=
-Internal {| fn_return := transBeePL_type (fd.(rtype)); 
-            fn_callconv := default_cc(fd); 
-            fn_params := zip (unzip1 (BeePL_mem.extract_list_rvtypes (fd.(args))))
-                             (typelist_list_type (transBeePL_types transBeePL_type 
-                               (unzip2 (BeePL_mem.extract_list_rvtypes (fd.(args))))));
-            fn_vars := zip (unzip1 (BeePL_mem.extract_list_rvtypes (fd.(lvars))))
-                             (typelist_list_type (transBeePL_types transBeePL_type 
-                               (unzip2 (BeePL_mem.extract_list_rvtypes (fd.(lvars))))));
-            fn_body := transBeePL_expr_st (fd.(body)) |}.
+(* Translates the BeePL function declaration to C function declaration *)
+(* For now we have only internal functions: later change it to include the case of external function *)
+Definition BeePLfd_function (fd : fun_decl) : res (Ctypes.fundef function) :=
+do crt <- transBeePL_type (fd.(rtype));
+do pt <- (transBeePL_types transBeePL_type (unzip2 (BeePL_mem.extract_list_rvtypes (fd.(args)))));
+do vt <- (transBeePL_types transBeePL_type (unzip2 (BeePL_mem.extract_list_rvtypes (fd.(lvars)))));
+do fbody <- transBeePL_expr_st (fd.(body));
+OK (Internal {| fn_return := crt; 
+                fn_callconv := default_cc(fd); 
+                fn_params := zip (unzip1 (BeePL_mem.extract_list_rvtypes (fd.(args))))
+                                 (typelist_list_type pt);
+                fn_vars := zip (unzip1 (BeePL_mem.extract_list_rvtypes (fd.(lvars))))
+                               (typelist_list_type vt);
+                fn_body :=  fbody|}).
 
+(* Translates the value that is assigned to global variable to C global variable data *)
 Definition gconstant_init_data (g : BeePL.gconstant) : init_data :=
 match g with 
 | Gvalue c => match c with 
@@ -276,33 +331,41 @@ match g with
 | Gspace z => Init_space z
 end. 
 
+(* Translates the list of global variable data to list of C global variable data *)
 Fixpoint gconstants_init_datas (gs : list BeePL.gconstant) : list init_data :=
 match gs with 
 | nil => nil
 | g :: gs => gconstant_init_data g :: gconstants_init_datas gs
 end. 
 
-Definition BeePLgd_gd (gv : globv) : globvar Ctypes.type  :=
-{| gvar_info := transBeePL_type (gv.(gtype)); 
-   gvar_init := gconstants_init_datas(gv.(gval)); 
-   gvar_readonly := false; 
-   gvar_volatile := false |}.
+(* Translates BeePL global variable to C global variable *)
+Definition BeePLgd_gd (gv : globv) : res (globvar Ctypes.type)  :=
+do gvt <- transBeePL_type (gv.(gtype));
+OK {| gvar_info := gvt; 
+      gvar_init := gconstants_init_datas(gv.(gval)); 
+      gvar_readonly := false; 
+      gvar_volatile := false |}.
 
-Definition BeePLdecl_gdef (d : BeePL.decl) : (globdef (Ctypes.fundef function) type) :=
+(* Translates a BeePL declaration to C declaration *)
+Definition BeePLdecl_gdef (d : BeePL.decl) : res (globdef (Ctypes.fundef function) type) :=
 match d with 
-| Fdecl fd => Gfun (BeePLfd_function fd)
-| Gvdecl gd => Gvar (BeePLgd_gd gd)
+| Fdecl fd => do cfd <- (BeePLfd_function fd); OK (Gfun cfd)
+| Gvdecl gd => do gv <- (BeePLgd_gd gd) ; OK (Gvar gv)
 (*| Tadecl ta => *) (* Fix me *)
 end.
 
+(* Translates a list of BeePL declarations to C declarations *)
 Fixpoint BeePLdecls_gdefs (ds : list BeePL.decl) : 
-list (globdef (Ctypes.fundef function) type) :=
+res (list (globdef (Ctypes.fundef function) type)) :=
 match ds with 
-| nil => nil
-| d :: ds => BeePLdecl_gdef d :: BeePLdecls_gdefs ds
+| nil => OK (nil)
+| d :: ds => do gd <- BeePLdecl_gdef d; 
+             do gds <- BeePLdecls_gdefs ds;
+             OK (gd :: gds)
 end.
 
 (* Fix me: I want to produce Csyntax.program *)  
-(* Missing compositie information and list of public functions *)
-Definition BeePL_compcert (m : BeePL.module) : (*Csyntax.program*) AST.program (Ctypes.fundef function) type :=
-  mkprogram (zip (unzip1 (fst (m))) (BeePLdecls_gdefs (unzip2 (fst(m))))) nil (snd(m)).
+(* Missing compositie information and list of public functions *) 
+Definition BeePL_compcert (m : BeePL.module) : res (AST.program (Ctypes.fundef function) type) :=
+do cfd <- (BeePLdecls_gdefs (unzip2 (fst(m))));
+ OK (mkprogram (zip (unzip1 (fst (m))) cfd) nil (snd(m))).
