cfrontend/BeePL_proof.v
@@ -95,9 +95,9 @@ End rel_type_ind.
 (***** Proof for correctness of type transformation *****)
 Fixpoint type_translated bt: 
 (forall ct, 
-transBeePL_type bt = ct ->
+transBeePL_type bt = OK ct ->
 rel_type bt ct) /\ (forall bts cts, 
-transBeePL_types transBeePL_type bts = cts ->
+transBeePL_types transBeePL_type bts = OK cts ->
 rel_types bts cts).
 Proof.
 destruct bt.
@@ -111,73 +111,84 @@ Admitted.
 From mathcomp Require Import all_ssreflect. 
 
 (****** Proof of correctness for transformation of operators ******)
-Lemma transl_notbool_cnotbool: forall v v' m t,
+Lemma transl_notbool_cnotbool: forall v v' m t ct,
 sem_unary_operation Notbool v t = Some v' -> 
-Cop.sem_unary_operation (transBeePL_uop_uop Notbool) (transBeePL_value_cvalue v) 
-     (transBeePL_type t) m = Some (transBeePL_value_cvalue v'). 
+transBeePL_type t = OK ct ->
+Cop.sem_unary_operation 
+ (transBeePL_uop_uop Notbool) (transBeePL_value_cvalue v) ct m = Some (transBeePL_value_cvalue v'). 
 Proof.
 intros; simpl. 
 generalize dependent (extract_type_notbool v t v' H). intros; subst; simpl.
 destruct v; inversion H; subst. destruct b.
 + unfold Cop.sem_notbool, Cop.bool_val; simpl. 
   assert (hneq : Int.eq (Int.repr 1) Int.zero = false).
-  ++ apply Int.eq_false; simpl. unfold not. intros. inversion H0.
-  ++ rewrite hneq; simpl. unfold Values.Vfalse, Int.zero. reflexivity.
+  ++ apply Int.eq_false; simpl. unfold not. intros. by inversion H0.
+  ++ rewrite hneq; simpl. unfold Values.Vfalse, Int.zero. 
+     rewrite /transBeePL_type in H0. case: H0; subst. by move=> <- /=. 
 + unfold Cop.sem_notbool, Cop.bool_val; simpl. 
   assert (hneq : Int.eq (Int.repr 0) Int.zero = true).
   ++ apply Int.eq_true; simpl. 
-  ++ rewrite hneq; simpl. unfold Values.Vtrue, Int.zero. reflexivity.
+  ++ rewrite hneq; simpl. unfold Values.Vtrue, Int.zero. 
+     rewrite /transBeePL_type in H0. case: H0; subst. by move=> <- /=. 
 Qed.
 
-Lemma transl_notint_cnotint: forall v v' m t,
+Lemma transl_notint_cnotint: forall v v' m t ct,
 sem_unary_operation Notint v t = Some v' -> 
-Cop.sem_unary_operation (transBeePL_uop_uop Notint) (transBeePL_value_cvalue v) 
-     (transBeePL_type t) m = Some (transBeePL_value_cvalue v'). 
+transBeePL_type t = OK ct ->
+Cop.sem_unary_operation 
+ (transBeePL_uop_uop Notint) (transBeePL_value_cvalue v) ct m = Some (transBeePL_value_cvalue v'). 
 Proof.
 intros; simpl.
 generalize dependent (extract_type_notint v t v' H). intros; subst; simpl.
-destruct H0; subst; destruct H0; subst.
+destruct H1; subst; destruct H1; subst.
 (* Int *)
 destruct v; inversion H; subst.
 unfold Cop.sem_notint, Int.zero, Int.not, Int.mone; simpl. 
-rewrite /transBeePL_isize_cisize. case: x H=> //= _. by case: x0=> //=.
+rewrite /transBeePL_isize_cisize. 
+rewrite /transBeePL_type in H0. case: H0; subst. move=> <- /=. 
+case: x H=> //= _. by case: x0=> //=.
 Qed.
 
-Lemma transl_neg_cneg: forall v v' m t,
-sem_unary_operation Neg v t = Some v' -> 
-Cop.sem_unary_operation (transBeePL_uop_uop Neg) (transBeePL_value_cvalue v) 
-     (transBeePL_type t) m = Some (transBeePL_value_cvalue v'). 
+Lemma transl_neg_cneg: forall v v' m t ct,
+sem_unary_operation Neg v t = Some v' ->
+transBeePL_type t = OK ct ->  
+Cop.sem_unary_operation 
+  (transBeePL_uop_uop Neg) (transBeePL_value_cvalue v) ct  m = Some (transBeePL_value_cvalue v'). 
 Proof.
 intros; simpl.
 generalize dependent (extract_type_neg v t v' H). intros; subst; simpl.
-destruct H0; subst; destruct H0; subst.
+destruct H1; subst; destruct H1; subst.
 (* Int *)
 destruct v; inversion H; subst.
 unfold Cop.sem_neg, Int.zero, Int.not, Int.mone; simpl. 
-rewrite /transBeePL_isize_cisize. case: x H=> //= _. by case: x0=> //=.
+rewrite /transBeePL_isize_cisize. rewrite /transBeePL_type in H0. 
+case: H0; subst. move=> <- /=. case: x H=> //= _. by case: x0=> //=.
 Qed.
 
-Lemma transl_uop_cuop : forall op v v' m t,
+Lemma transl_uop_cuop : forall op v v' m t ct,
 sem_unary_operation op v t = Some v' -> 
-Cop.sem_unary_operation (transBeePL_uop_uop op) (transBeePL_value_cvalue v) (transBeePL_type t) m = 
-Some (transBeePL_value_cvalue v').
+transBeePL_type t = OK ct ->
+Cop.sem_unary_operation 
+ (transBeePL_uop_uop op) (transBeePL_value_cvalue v) ct m = Some (transBeePL_value_cvalue v').
 Proof.
 intros. destruct op; simpl; auto; subst.
 (* Notbool *)
-+ generalize dependent (transl_notbool_cnotbool v v' m t H). intros. apply H0.
++ by generalize dependent (transl_notbool_cnotbool v v' m t ct H H0). 
 (* Notint *)
-+ generalize dependent (transl_notint_cnotint v v' m t H). intros. apply H0.
++ by generalize dependent (transl_notint_cnotint v v' m t ct H H0). 
 (* Neg *)
-+ generalize dependent (transl_neg_cneg v v' m t H). intros. apply H0.
++ by generalize dependent (transl_neg_cneg v v' m t ct H H0).
 Qed.
 
-Lemma transl_plus_cadd: forall v1 v2 t1 t2 v cenv m,
+Lemma transl_plus_cadd: forall v1 v2 t1 t2 v cenv m ct1 ct2,
 sem_binary_operation Plus v1 v2 t1 t2 = Some v -> 
-Cop.sem_binary_operation cenv (transBeePL_bop_bop Plus) (transBeePL_value_cvalue v1) 
-     (transBeePL_type t1) (transBeePL_value_cvalue v2) (transBeePL_type t2) m = 
+transBeePL_type t1 = OK ct1 ->
+transBeePL_type t2 = OK ct2 ->
+Cop.sem_binary_operation cenv 
+  (transBeePL_bop_bop Plus) (transBeePL_value_cvalue v1) ct1 (transBeePL_value_cvalue v2) ct2 m = 
 Some (transBeePL_value_cvalue v). 
 Proof.
-move=> v1 v2 t1 t2 v cenv m hs. 
+move=> v1 v2 t1 t2 v cenv m ct1 ct2 hs. 
 have [sz [s ht]] := extract_type_plus1 v1 v2 t1 t2 v hs; subst.
 rewrite /sem_binary_operation /sem_plus /= in hs. move: hs.
 rewrite /Cop.sem_binary_operation /= /Cop.sem_add /= /transBeePL_isize_cisize /transBeePL_sign_csign.
@@ -187,26 +198,26 @@ case: v1=> //=.
   move=> [] hv; subst. case: sz=> //=.
   + case: s=> //=.
     + rewrite /Cop.classify_add /= /Cop.sem_binarith /= /Cop.sem_cast /= /Cop.classify_cast /=. 
-      case: sz'=> //=. by case: s'=> //=.
+      move=> [] <- /= [] <- /=. case: sz'=> //=. by case: s'=> //=.
     + rewrite /Cop.classify_add /= /Cop.sem_binarith /= /Cop.sem_cast /= /Cop.classify_cast /=. 
-      case: sz'=> //=. by case: s'=> //=.
+      move=> [] <- /= [] <- /=. case: sz'=> //=. by case: s'=> //=.
     + rewrite /Cop.classify_add /= /Cop.sem_binarith /= /Cop.sem_cast /= /Cop.classify_cast /=. 
-      case: sz'=> //=. by case: s'=> //=.
+      move=> [] <- /= [] <- /=. case: sz'=> //=. by case: s'=> //=.
     + rewrite /Cop.classify_add /= /Cop.sem_binarith /= /Cop.sem_cast /= /Cop.classify_cast /=. 
-      case: sz'=> //=. by case: s=> //=.
-    rewrite /Cop.classify_add /= /Cop.sem_binarith /= /Cop.sem_cast /= /Cop.classify_cast /=. 
-    case: s=> //=. case: s=> //=. by case: s'=> //=.
+      move=> [] <- /= [] <- /=. case: sz'=> //=;case: s=> //=. by case: s'=> //=. 
   by case: v2=> //=.
 by case: v2=> //=.
 Qed.
 
-Lemma transl_minus_csub: forall v1 v2 t1 t2 v cenv m,
+Lemma transl_minus_csub: forall v1 v2 t1 t2 v cenv m ct1 ct2,
 sem_binary_operation Minus v1 v2 t1 t2 = Some v -> 
-Cop.sem_binary_operation cenv (transBeePL_bop_bop Minus) (transBeePL_value_cvalue v1) 
-     (transBeePL_type t1) (transBeePL_value_cvalue v2) (transBeePL_type t2) m = 
+transBeePL_type t1 = OK ct1 ->
+transBeePL_type t2 = OK ct2 ->
+Cop.sem_binary_operation cenv 
+  (transBeePL_bop_bop Minus) (transBeePL_value_cvalue v1) ct1 (transBeePL_value_cvalue v2) ct2 m = 
 Some (transBeePL_value_cvalue v). 
 Proof.
-move=> v1 v2 t1 t2 v cenv m hs. 
+move=> v1 v2 t1 t2 v cenv m ct1 ct2 hs. 
 have [sz [s ht]] := extract_type_minus1 v1 v2 t1 t2 v hs; subst.
 rewrite /sem_binary_operation /sem_minus /= in hs. move: hs.
 rewrite /Cop.sem_binary_operation /= /Cop.sem_sub /= /transBeePL_isize_cisize /transBeePL_sign_csign.
@@ -216,26 +227,26 @@ case: v1=> //=.
   move=> [] hv; subst. case: sz=> //=.
   + case: s=> //=.
     + rewrite /Cop.classify_add /= /Cop.sem_binarith /= /Cop.sem_cast /= /Cop.classify_cast /=. 
-      case: sz'=> //=. by case: s'=> //=.
+      move=> [] <- /= [] <- /=. case: sz'=> //=. by case: s'=> //=.
     + rewrite /Cop.classify_add /= /Cop.sem_binarith /= /Cop.sem_cast /= /Cop.classify_cast /=. 
-      case: sz'=> //=. by case: s'=> //=.
+      move=> [] <- /= [] <- /=. case: sz'=> //=. by case: s'=> //=.
     + rewrite /Cop.classify_add /= /Cop.sem_binarith /= /Cop.sem_cast /= /Cop.classify_cast /=. 
-      case: sz'=> //=. by case: s'=> //=.
+      move=> [] <- /= [] <- /=. case: sz'=> //=. by case: s'=> //=.
     + rewrite /Cop.classify_add /= /Cop.sem_binarith /= /Cop.sem_cast /= /Cop.classify_cast /=. 
-      case: sz'=> //=. by case: s=> //=.
-    rewrite /Cop.classify_add /= /Cop.sem_binarith /= /Cop.sem_cast /= /Cop.classify_cast /=. 
-    case: s=> //=. case: s=> //=. by case: s'=> //=.
+      move=> [] <- /= [] <- /=. case: sz'=> //=;case: s=> //=. by case: s'=> //=. 
   by case: v2=> //=.
 by case: v2=> //=.
 Qed.
 
-Lemma transl_mult_cmul: forall v1 v2 t1 t2 v cenv m,
+Lemma transl_mult_cmul: forall v1 v2 t1 t2 v cenv m ct1 ct2,
 sem_binary_operation Mult v1 v2 t1 t2 = Some v -> 
-Cop.sem_binary_operation cenv (transBeePL_bop_bop Mult) (transBeePL_value_cvalue v1) 
-     (transBeePL_type t1) (transBeePL_value_cvalue v2) (transBeePL_type t2) m = 
+transBeePL_type t1 = OK ct1 ->
+transBeePL_type t2 = OK ct2 ->
+Cop.sem_binary_operation cenv 
+  (transBeePL_bop_bop Mult) (transBeePL_value_cvalue v1) ct1 (transBeePL_value_cvalue v2) ct2 m = 
 Some (transBeePL_value_cvalue v). 
 Proof.
-move=> v1 v2 t1 t2 v cenv m hs. 
+move=> v1 v2 t1 t2 v cenv m ct1 ct2 hs. 
 have [sz [s ht]] := extract_type_mult1 v1 v2 t1 t2 v hs; subst.
 rewrite /sem_binary_operation /sem_mult /= in hs. move: hs.
 rewrite /Cop.sem_binary_operation /= /Cop.sem_mul /= /transBeePL_isize_cisize /transBeePL_sign_csign.
@@ -245,15 +256,13 @@ case: v1=> //=.
   move=> [] hv; subst. case: sz=> //=.
   + case: s=> //=.
     + rewrite /Cop.classify_add /= /Cop.sem_binarith /= /Cop.sem_cast /= /Cop.classify_cast /=. 
-      case: sz'=> //=. by case: s'=> //=.
+      move=> [] <- /= [] <- /=. case: sz'=> //=. by case: s'=> //=.
     + rewrite /Cop.classify_add /= /Cop.sem_binarith /= /Cop.sem_cast /= /Cop.classify_cast /=. 
-      case: sz'=> //=. by case: s'=> //=.
+      move=> [] <- /= [] <- /=. case: sz'=> //=. by case: s'=> //=.
     + rewrite /Cop.classify_add /= /Cop.sem_binarith /= /Cop.sem_cast /= /Cop.classify_cast /=. 
-      case: sz'=> //=. by case: s'=> //=.
+      move=> [] <- /= [] <- /=. case: sz'=> //=. by case: s'=> //=.
     + rewrite /Cop.classify_add /= /Cop.sem_binarith /= /Cop.sem_cast /= /Cop.classify_cast /=. 
-      case: sz'=> //=. by case: s=> //=.
-    rewrite /Cop.classify_add /= /Cop.sem_binarith /= /Cop.sem_cast /= /Cop.classify_cast /=. 
-    case: s=> //=. case: s=> //=. by case: s'=> //=.
+      move=> [] <- /= [] <- /=. case: sz'=> //=;case: s=> //=. by case: s'=> //=. 
   by case: v2=> //=.
 by case: v2=> //=.
 Qed.
@@ -272,13 +281,15 @@ Proof.
 move=> s. by case: s=> //=.
 Qed.
 
-Lemma transl_div_cdiv: forall v1 v2 t1 t2 v cenv m,
+Lemma transl_div_cdiv: forall v1 v2 t1 t2 v cenv m ct1 ct2,
 sem_binary_operation Div v1 v2 t1 t2 = Some v -> 
-Cop.sem_binary_operation cenv (transBeePL_bop_bop Div) (transBeePL_value_cvalue v1) 
-     (transBeePL_type t1) (transBeePL_value_cvalue v2) (transBeePL_type t2) m = 
+transBeePL_type t1 = OK ct1 ->
+transBeePL_type t2 = OK ct2 ->
+Cop.sem_binary_operation cenv 
+ (transBeePL_bop_bop Div) (transBeePL_value_cvalue v1) ct1 (transBeePL_value_cvalue v2) ct2 m = 
 Some (transBeePL_value_cvalue v). 
 Proof.
-move=> v1 v2 t1 t2 v cenv m hs.
+move=> v1 v2 t1 t2 v cenv m ct1 ct2 hs.
 have [sz [s ht]] := extract_type_div1 v1 v2 t1 t2 v hs; subst.
 have [sz' [s' ht]] := extract_type_div2 v1 v2 (Ptype (Tint sz s)) t2 v hs; subst.
 inversion hs; subst. case: s hs H0=> //= hs _.
@@ -293,10 +304,10 @@ inversion hs; subst. case: s hs H0=> //= hs _.
       case: ifP=> //= hi'. 
       + case: ifP=> //= hi.
         + by rewrite hi /= in h.
-        rewrite hi /= in h. case: ifP=> //=. by rewrite hi h.
+        rewrite hi /= in h. move=> [] <- /= [] <- /=. case: ifP=> //=. by rewrite hi h.
       case: ifP=> //= hi.
       + by rewrite hi /= in h.
-      rewrite hi /= in h. case: ifP=> //=. by rewrite hi h.
+      rewrite hi /= in h. move=> [] <- /= [] <- /=. case: ifP=> //=. by rewrite hi h.
     by case: v2=> //=.
   by case: v2=> //=.
  case:v1=> //=.
@@ -320,20 +331,22 @@ case: v1=> //=.
   rewrite /Cop.sem_div /Cop.sem_binarith /= /Cop.sem_cast /=.
   case: ifP=> //= hi'.
   + case: ifP=> //= hi1. + by rewrite hi1 in hi.
-    case: ifP=> //= hi2. by rewrite hi2 in hi.
+    move=> [] <- /= [] <- /=. case: ifP=> //= hi2. by rewrite hi2 in hi.
   case: ifP=> //= hi1. + by rewrite hi1 in hi.
-  case: ifP=> //= hi2. by rewrite hi in hi2.
+  move=> [] <- /= [] <- /=. case: ifP=> //= hi2. by rewrite hi in hi2.
 + by case: v2=> //=.
 by case: v2=> //=.
 Qed.
 
-Lemma transl_and_cand: forall v1 v2 t1 t2 v cenv m,
+Lemma transl_and_cand: forall v1 v2 t1 t2 v cenv m ct1 ct2,
 sem_binary_operation And v1 v2 t1 t2 = Some v -> 
-Cop.sem_binary_operation cenv (transBeePL_bop_bop And) (transBeePL_value_cvalue v1) 
-     (transBeePL_type t1) (transBeePL_value_cvalue v2) (transBeePL_type t2) m = 
+transBeePL_type t1 = OK ct1 ->
+transBeePL_type t2 = OK ct2 ->
+Cop.sem_binary_operation cenv 
+  (transBeePL_bop_bop And) (transBeePL_value_cvalue v1) ct1 (transBeePL_value_cvalue v2) ct2 m = 
 Some (transBeePL_value_cvalue v). 
 Proof.
-move=> v1 v2 t1 t2 v cenv m /= ha. case: v1 ha=> //=.
+move=> v1 v2 t1 t2 v cenv m ct1 ct2 /= ha. case: v1 ha=> //=.
 + case: v2=> //=. case: t1=> //= p. case: p=> //=.
   case: t2=> //= p. by case: p=> //=.
 + case: v2=> //= i i'. case: t1=> //= p. case: p=> //=.
@@ -341,7 +354,7 @@ move=> v1 v2 t1 t2 v cenv m /= ha. case: v1 ha=> //=.
 + case: v2=> //= b b'. case: t1=> //= p. case: p=> //=.
   case: t2=> //= p. case: p=> //= [] [] hv; subst; rewrite /=.
   rewrite /Cop.sem_and /Cop.sem_binarith /Cop.sem_cast /=.
-  case: Archi.ptr64=> //=.
+  move=> [] <- /= [] <- /=. case: Archi.ptr64=> //=.
   + case: b'=> //=. by case: b=> //=.
   case: (intsize_eq Ctypes.I32 Ctypes.I32) => //= heq.  
   case: b'=> //=. by case: b=> //=.
@@ -350,13 +363,15 @@ case: p''=> //=. case: t2=> //= i' b. case:b=> //= p''.
 by case:p''=> //=.
 Qed.
 
-Lemma transl_or_cor: forall v1 v2 t1 t2 v cenv m,
+Lemma transl_or_cor: forall v1 v2 t1 t2 v cenv m ct1 ct2,
 sem_binary_operation Or v1 v2 t1 t2 = Some v -> 
-Cop.sem_binary_operation cenv (transBeePL_bop_bop Or) (transBeePL_value_cvalue v1) 
-     (transBeePL_type t1) (transBeePL_value_cvalue v2) (transBeePL_type t2) m = 
+transBeePL_type t1 = OK ct1 ->
+transBeePL_type t2 = OK ct2 ->
+Cop.sem_binary_operation cenv 
+  (transBeePL_bop_bop Or) (transBeePL_value_cvalue v1) ct1 (transBeePL_value_cvalue v2) ct2 m = 
 Some (transBeePL_value_cvalue v). 
 Proof.
-move=> v1 v2 t1 t2 v cenv m /= ha. case: v1 ha=> //=.
+move=> v1 v2 t1 t2 v cenv m ct1 ct2 /= ha. case: v1 ha=> //=.
 + case: v2=> //=. case: t1=> //= p. case: p=> //=.
   case: t2=> //= p. by case: p=> //=.
 + case: v2=> //= i i'. case: t1=> //= p. case: p=> //=.
@@ -364,7 +379,7 @@ move=> v1 v2 t1 t2 v cenv m /= ha. case: v1 ha=> //=.
 + case: v2=> //= b b'. case: t1=> //= p. case: p=> //=.
   case: t2=> //= p. case: p=> //= [] [] hv; subst; rewrite /=.
   rewrite /Cop.sem_or /Cop.sem_binarith /Cop.sem_cast /=.
-  case: Archi.ptr64=> //=.
+  move=> [] <- /= [] <- /=. case: Archi.ptr64=> //=.
   + case: b'=> //=. by case: b=> //=.
   by case: b=> //=.
   case: (intsize_eq Ctypes.I32 Ctypes.I32) => //= heq.  
@@ -375,21 +390,23 @@ case: p''=> //=. case: t2=> //= i' b. case:b=> //= p''.
 by case:p''=> //=.
 Qed.
 
-Lemma transl_xor_cxor: forall v1 v2 t1 t2 v cenv m,
+Lemma transl_xor_cxor: forall v1 v2 t1 t2 v cenv m ct1 ct2,
 sem_binary_operation Xor v1 v2 t1 t2 = Some v -> 
-Cop.sem_binary_operation cenv (transBeePL_bop_bop Xor) (transBeePL_value_cvalue v1) 
-     (transBeePL_type t1) (transBeePL_value_cvalue v2) (transBeePL_type t2) m = 
+transBeePL_type t1 = OK ct1 ->
+transBeePL_type t2 = OK ct2 ->
+Cop.sem_binary_operation cenv 
+  (transBeePL_bop_bop Xor) (transBeePL_value_cvalue v1) ct1 (transBeePL_value_cvalue v2) ct2 m = 
 Some (transBeePL_value_cvalue v). 
 Proof.
-move=> v1 v2 t1 t2 v cenv m /= ha. case: v1 ha=> //=.
+move=> v1 v2 t1 t2 v cenv m ct1 ct2 /= ha. case: v1 ha=> //=.
 + case: v2=> //=. case: t1=> //= p. case: p=> //=.
   case: t2=> //= p. by case: p=> //=.
 + case: v2=> //= i i'. case: t1=> //= p. case: p=> //=.
   case: t2=> //= p. by case: p=> //=.
 + case: v2=> //= b b'. case: t1=> //= p. case: p=> //=.
   case: t2=> //= p. case: p=> //= [] [] hv; subst; rewrite /=.
-  rewrite /Cop.sem_or /Cop.sem_binarith /Cop.sem_cast /=.
-  case: Archi.ptr64=> //=.
+  rewrite /Cop.sem_xor /Cop.sem_binarith /Cop.sem_cast /=.
+  move=> [] <- /= [] <- /=. case: Archi.ptr64=> //=.
   + case: b'=> //=. by case: b=> //=.
   by case: b=> //=.
   case: (intsize_eq Ctypes.I32 Ctypes.I32) => //= heq.  
@@ -400,31 +417,35 @@ case: p''=> //=. case: t2=> //= i' b. case:b=> //= p''.
 by case:p''=> //=.
 Qed.
 
-Lemma transl_shl_cshl: forall v1 v2 t1 t2 v cenv m,
+Lemma transl_shl_cshl: forall v1 v2 t1 t2 v cenv m ct1 ct2,
 sem_binary_operation Shl v1 v2 t1 t2 = Some v -> 
-Cop.sem_binary_operation cenv (transBeePL_bop_bop Shl) (transBeePL_value_cvalue v1) 
-     (transBeePL_type t1) (transBeePL_value_cvalue v2) (transBeePL_type t2) m = 
+transBeePL_type t1 = OK ct1 ->
+transBeePL_type t2 = OK ct2 ->
+Cop.sem_binary_operation cenv 
+ (transBeePL_bop_bop Shl) (transBeePL_value_cvalue v1) ct1 (transBeePL_value_cvalue v2) ct2 m = 
 Some (transBeePL_value_cvalue v). 
 Proof.
-move=> v1 v2 t1 t2 v cenv m hs. 
+move=> v1 v2 t1 t2 v cenv m ct1 ct2 hs. 
 have [sz [s ht]] := extract_type_shl1 v1 v2 t1 t2 v hs; subst.
 have [sz' [s' ht]] := extract_type_shl2 v1 v2 (Ptype (Tint sz s)) t2 v hs; subst.
 case: v1 hs=> //=.
 + by case: v2=> //=.
 + case: v2=> //= i i'. case: sz=> //=. case: sz'=> //=.
   case: ifP=> //= hl [] hv; subst. rewrite /Cop.sem_shl /Cop.sem_shift /=. 
-  rewrite hl /= /Cop.classify_shift /=. by case: s=> //=.
+  rewrite hl /= /Cop.classify_shift /=. move=> [] <- /= [] <- /=. by case: s=> //=.
 + by case: v2=> //=.
 by case: v2=> //=.
 Qed.
 
-Lemma transl_shr_cshr: forall v1 v2 t1 t2 v cenv m,
+Lemma transl_shr_cshr: forall v1 v2 t1 t2 v cenv m ct1 ct2,
 sem_binary_operation Shr v1 v2 t1 t2 = Some v -> 
-Cop.sem_binary_operation cenv (transBeePL_bop_bop Shr) (transBeePL_value_cvalue v1) 
-     (transBeePL_type t1) (transBeePL_value_cvalue v2) (transBeePL_type t2) m = 
+transBeePL_type t1 = OK ct1 ->
+transBeePL_type t2 = OK ct2 ->
+Cop.sem_binary_operation cenv 
+ (transBeePL_bop_bop Shr) (transBeePL_value_cvalue v1) ct1 (transBeePL_value_cvalue v2) ct2 m = 
 Some (transBeePL_value_cvalue v). 
 Proof.
-move=> v1 v2 t1 t2 v cenv m hs.
+move=> v1 v2 t1 t2 v cenv m ct1 ct2 hs.
 have [s ht] := extract_type_shr1 v1 v2 t1 t2 v hs; subst.
 have [s' ht] := extract_type_shr2 v1 v2 (Ptype (Tint I32 s)) t2 v hs; subst.
 inversion hs; subst. case: s hs H0=> //= hs _.
@@ -435,7 +456,7 @@ inversion hs; subst. case: s hs H0=> //= hs _.
     + by case: v2=> //=.
     + case: v2=> //= i i'. case: ifP=> //= hl [] hv; subst.
       rewrite /Cop.sem_shr /Cop.sem_binarith /= /Cop.sem_shift /=.
-      by rewrite hl /=.
+      move=> [] <- /= [] <- /=. by rewrite hl /=.
     by case: v2=> //=.
   by case: v2=> //=.
  case:v1=> //=.
@@ -456,22 +477,24 @@ case: v1=> //=.
 + by case: v2=> //=.
 + case: v2=> //= i i'. case: ifP=> //= hl [] hv; subst.
   rewrite /Cop.sem_shr /Cop.sem_binarith /= /Cop.sem_shift /=.
-  by rewrite hl /=.
+  move=> [] <- /= [] <- /=. by rewrite hl /=.
 + by case: v2=> //=.
 by case: v2=> //=.
 Qed.
 
-Lemma transl_eq_ceq: forall v1 v2 t1 t2 v cenv m,
+Lemma transl_eq_ceq: forall v1 v2 t1 t2 v cenv m ct1 ct2,
 sem_binary_operation Eq v1 v2 t1 t2 = Some v -> 
-Cop.sem_binary_operation cenv (transBeePL_bop_bop Eq) (transBeePL_value_cvalue v1) 
-     (transBeePL_type t1) (transBeePL_value_cvalue v2) (transBeePL_type t2) m = 
+transBeePL_type t1 = OK ct1 ->
+transBeePL_type t2 = OK ct2 ->
+Cop.sem_binary_operation cenv 
+  (transBeePL_bop_bop Eq) (transBeePL_value_cvalue v1) ct1 (transBeePL_value_cvalue v2) ct2 m = 
 Some (transBeePL_value_cvalue v). 
 Proof.
-move=> v1 v2 t1 t2 v cenv m /= ha. case: v1 ha=> //=.
+move=> v1 v2 t1 t2 v cenv m ct1 ct2 /= ha. case: v1 ha=> //=.
 + case: v2=> //=. case: t1=> //= p. case: p=> //=.
   case: t2=> //= p. case: p=> //= [] [] hv; subst; rewrite /=.
   rewrite /Cop.sem_cmp /Cop.sem_binarith /Cop.sem_cast /=. 
-  by case: (Archi.ptr64)=> //=.
+  move=> [] <- /= [] <- /=. by case: (Archi.ptr64)=> //=.
 + case: v2=> //=. case: t1=> //= p. case: p=> //=.
   case: t2=> //= p. case: p=> //= sz s sz' s' i i'. 
   case: s'=> //=.
@@ -479,20 +502,20 @@ move=> v1 v2 t1 t2 v cenv m /= ha. case: v1 ha=> //=.
     rewrite /Cop.sem_cmp /= /Cop.sem_binarith /= /Cop.sem_cast /=.
     case: ifP=> //= hi.
     + case: ifP=> //= hi'.
-      + case: Archi.ptr64=>//=.
+      + move=> [] <- /= [] <- /=. case: Archi.ptr64=>//=.
         + rewrite /Values.Val.of_bool /bool_to_int /=. by case: ifP=> //=.
         case: (intsize_eq Ctypes.I32 Ctypes.I32)=> //= heq.
         rewrite /Values.Val.of_bool /bool_to_int /=. by case: ifP=> //=.
-      case: Archi.ptr64=>//=.
+      move=> [] <- /= [] <- /=. case: Archi.ptr64=>//=.
       + rewrite /Values.Val.of_bool /bool_to_int /=. by case: ifP=> //=.
       case: (intsize_eq Ctypes.I32 Ctypes.I32)=> //= heq.
       rewrite /Values.Val.of_bool /bool_to_int /=. by case: ifP=> //=.
       case: ifP=> //= hi1.
-      + case: Archi.ptr64=>//=.
+      + move=> [] <- /= [] <- /=. case: Archi.ptr64=>//=.
         + rewrite /Values.Val.of_bool /bool_to_int /=. by case: ifP=> //=.
         case: (intsize_eq Ctypes.I32 Ctypes.I32)=> //= heq.
         rewrite /Values.Val.of_bool /bool_to_int /=. by case: ifP=> //=.
-      case: Archi.ptr64=>//=.
+      move=> [] <- /= [] <- /=. case: Archi.ptr64=>//=.
       + rewrite /Values.Val.of_bool /bool_to_int /=. by case: ifP=> //=.
       case: (intsize_eq Ctypes.I32 Ctypes.I32)=> //= heq.
       rewrite /Values.Val.of_bool /bool_to_int /=. by case: ifP=> //=.
@@ -500,26 +523,26 @@ move=> v1 v2 t1 t2 v cenv m /= ha. case: v1 ha=> //=.
    rewrite /Cop.sem_cmp /= /Cop.sem_binarith /= /Cop.sem_cast /=.
     case: ifP=> //= hi.
     + case: ifP=> //= hi'.
-      + case: Archi.ptr64=>//=.
+      + move=> [] <- /= [] <- /=. case: Archi.ptr64=>//=.
         + rewrite /Values.Val.of_bool /bool_to_int /=. by case: ifP=> //=.
         case: (intsize_eq Ctypes.I32 Ctypes.I32)=> //= heq.
         rewrite /Values.Val.of_bool /bool_to_int /=. by case: ifP=> //=.
-      case: Archi.ptr64=>//=.
+      move=> [] <- /= [] <- /=. case: Archi.ptr64=>//=.
       + rewrite /Values.Val.of_bool /bool_to_int /=. by case: ifP=> //=.
       case: (intsize_eq Ctypes.I32 Ctypes.I32)=> //= heq.
       rewrite /Values.Val.of_bool /bool_to_int /=. by case: ifP=> //=.
       case: ifP=> //= hi1.
-      + case: Archi.ptr64=>//=.
+      + move=> [] <- /= [] <- /=. case: Archi.ptr64=>//=.
         + rewrite /Values.Val.of_bool /bool_to_int /=. by case: ifP=> //=.
         case: (intsize_eq Ctypes.I32 Ctypes.I32)=> //= heq.
         rewrite /Values.Val.of_bool /bool_to_int /=. by case: ifP=> //=.
-      case: Archi.ptr64=>//=.
+      move=> [] <- /= [] <- /=. case: Archi.ptr64=>//=.
       + rewrite /Values.Val.of_bool /bool_to_int /=. by case: ifP=> //=.
       case: (intsize_eq Ctypes.I32 Ctypes.I32)=> //= heq.
       rewrite /Values.Val.of_bool /bool_to_int /=. by case: ifP=> //=.
   case: v2=> //=. case: t1=> //= p. case: p=> //=. case: t2=> //= p.
   case: p=> //= b b' [] hv; subst. rewrite /Cop.sem_cmp /= /Cop.sem_binarith /= /Cop.sem_cast /=.
-  case: Archi.ptr64=> //=.
+  move=> [] <- /= [] <- /=. case: Archi.ptr64=> //=.
   + rewrite /Values.Val.of_bool /bool_to_int. case: ifP=> //=.
     + case: ifP=> //= _. 
       + by case: ifP=> //=.
@@ -544,17 +567,19 @@ case: p''=> //= sz s. case: t2=> //= b' b''. case: b''=> //= p1.
 by case: p1=> //=.
 Qed.
 
-Lemma transl_neq_cneq: forall v1 v2 t1 t2 v cenv m,
-sem_binary_operation Neq v1 v2 t1 t2 = Some v -> 
-Cop.sem_binary_operation cenv (transBeePL_bop_bop Neq) (transBeePL_value_cvalue v1) 
-     (transBeePL_type t1) (transBeePL_value_cvalue v2) (transBeePL_type t2) m = 
+Lemma transl_neq_cneq: forall v1 v2 t1 t2 v cenv m ct1 ct2,
+sem_binary_operation Neq v1 v2 t1 t2 = Some v ->
+transBeePL_type t1 = OK ct1 ->
+transBeePL_type t2 = OK ct2 -> 
+Cop.sem_binary_operation cenv 
+  (transBeePL_bop_bop Neq) (transBeePL_value_cvalue v1) ct1 (transBeePL_value_cvalue v2) ct2 m = 
 Some (transBeePL_value_cvalue v). 
 Proof.
-move=> v1 v2 t1 t2 v cenv m /= ha. case: v1 ha=> //=.
+move=> v1 v2 t1 t2 v cenv m ct1 ct2 /= ha. case: v1 ha=> //=.
 + case: v2=> //=. case: t1=> //= p. case: p=> //=.
   case: t2=> //= p. case: p=> //= [] [] hv; subst; rewrite /=.
-  rewrite /Cop.sem_cmp /Cop.sem_binarith /Cop.sem_cast /=. 
-  by case: (Archi.ptr64)=> //=.
+  rewrite /Cop.sem_cmp /Cop.sem_binarith /Cop.sem_cast /=.  
+  move=> [] <- /= [] <- /=. by case: (Archi.ptr64)=> //=.
 + case: v2=> //=. case: t1=> //= p. case: p=> //=.
   case: t2=> //= p. case: p=> //= sz s sz' s' i i'. 
   case: s'=> //=.
@@ -562,20 +587,20 @@ move=> v1 v2 t1 t2 v cenv m /= ha. case: v1 ha=> //=.
     rewrite /Cop.sem_cmp /= /Cop.sem_binarith /= /Cop.sem_cast /=.
     case: ifP=> //= hi.
     + case: ifP=> //= hi'.
-      + case: Archi.ptr64=>//=.
+      + move=> [] <- /= [] <- /=. case: Archi.ptr64=>//=.
         + rewrite /Values.Val.of_bool /bool_to_int /=. by case: ifP=> //=.
         case: (intsize_eq Ctypes.I32 Ctypes.I32)=> //= heq.
         rewrite /Values.Val.of_bool /bool_to_int /=. by case: ifP=> //=.
-      case: Archi.ptr64=>//=.
+      move=> [] <- /= [] <- /=. case: Archi.ptr64=>//=.
       + rewrite /Values.Val.of_bool /bool_to_int /=. by case: ifP=> //=.
       case: (intsize_eq Ctypes.I32 Ctypes.I32)=> //= heq.
       rewrite /Values.Val.of_bool /bool_to_int /=. by case: ifP=> //=.
       case: ifP=> //= hi1.
-      + case: Archi.ptr64=>//=.
+      + move=> [] <- /= [] <- /=. case: Archi.ptr64=>//=.
         + rewrite /Values.Val.of_bool /bool_to_int /=. by case: ifP=> //=.
         case: (intsize_eq Ctypes.I32 Ctypes.I32)=> //= heq.
         rewrite /Values.Val.of_bool /bool_to_int /=. by case: ifP=> //=.
-      case: Archi.ptr64=>//=.
+      move=> [] <- /= [] <- /=. case: Archi.ptr64=>//=.
       + rewrite /Values.Val.of_bool /bool_to_int /=. by case: ifP=> //=.
       case: (intsize_eq Ctypes.I32 Ctypes.I32)=> //= heq.
       rewrite /Values.Val.of_bool /bool_to_int /=. by case: ifP=> //=.
@@ -583,26 +608,26 @@ move=> v1 v2 t1 t2 v cenv m /= ha. case: v1 ha=> //=.
    rewrite /Cop.sem_cmp /= /Cop.sem_binarith /= /Cop.sem_cast /=.
     case: ifP=> //= hi.
     + case: ifP=> //= hi'.
-      + case: Archi.ptr64=>//=.
+      + move=> [] <- /= [] <- /=. case: Archi.ptr64=>//=.
         + rewrite /Values.Val.of_bool /bool_to_int /=. by case: ifP=> //=.
         case: (intsize_eq Ctypes.I32 Ctypes.I32)=> //= heq.
         rewrite /Values.Val.of_bool /bool_to_int /=. by case: ifP=> //=.
-      case: Archi.ptr64=>//=.
+      move=> [] <- /= [] <- /=. case: Archi.ptr64=>//=.
       + rewrite /Values.Val.of_bool /bool_to_int /=. by case: ifP=> //=.
       case: (intsize_eq Ctypes.I32 Ctypes.I32)=> //= heq.
       rewrite /Values.Val.of_bool /bool_to_int /=. by case: ifP=> //=.
       case: ifP=> //= hi1.
-      + case: Archi.ptr64=>//=.
+      + move=> [] <- /= [] <- /=. case: Archi.ptr64=>//=.
         + rewrite /Values.Val.of_bool /bool_to_int /=. by case: ifP=> //=.
         case: (intsize_eq Ctypes.I32 Ctypes.I32)=> //= heq.
         rewrite /Values.Val.of_bool /bool_to_int /=. by case: ifP=> //=.
-      case: Archi.ptr64=>//=.
+      move=> [] <- /= [] <- /=. case: Archi.ptr64=>//=.
       + rewrite /Values.Val.of_bool /bool_to_int /=. by case: ifP=> //=.
       case: (intsize_eq Ctypes.I32 Ctypes.I32)=> //= heq.
       rewrite /Values.Val.of_bool /bool_to_int /=. by case: ifP=> //=.
   case: v2=> //=. case: t1=> //= p. case: p=> //=. case: t2=> //= p.
   case: p=> //= b b' [] hv; subst. rewrite /Cop.sem_cmp /= /Cop.sem_binarith /= /Cop.sem_cast /=.
-  case: Archi.ptr64=> //=.
+  move=> [] <- /= [] <- /=. case: Archi.ptr64=> //=.
   + rewrite /Values.Val.of_bool /bool_to_int. case: ifP=> //=.
     + case: ifP=> //= _. 
       + by case: ifP=> //=.
@@ -627,17 +652,19 @@ case: p''=> //= sz s. case: t2=> //= b' b''. case: b''=> //= p1.
 by case: p1=> //=.
 Qed.
 
-Lemma transl_lt_clt: forall v1 v2 t1 t2 v cenv m,
+Lemma transl_lt_clt: forall v1 v2 t1 t2 v cenv m ct1 ct2,
 sem_binary_operation Lt v1 v2 t1 t2 = Some v -> 
-Cop.sem_binary_operation cenv (transBeePL_bop_bop Lt) (transBeePL_value_cvalue v1) 
-     (transBeePL_type t1) (transBeePL_value_cvalue v2) (transBeePL_type t2) m = 
+transBeePL_type t1 = OK ct1 ->
+transBeePL_type t2 = OK ct2 -> 
+Cop.sem_binary_operation cenv 
+  (transBeePL_bop_bop Lt) (transBeePL_value_cvalue v1) ct1 (transBeePL_value_cvalue v2) ct2 m = 
 Some (transBeePL_value_cvalue v). 
 Proof.
-move=> v1 v2 t1 t2 v cenv m /= ha. case: v1 ha=> //=.
+move=> v1 v2 t1 t2 v cenv m ct1 ct2 /= ha. case: v1 ha=> //=.
 + case: v2=> //=. case: t1=> //= p. case: p=> //=.
   case: t2=> //= p. case: p=> //= [] [] hv; subst; rewrite /=.
   rewrite /Cop.sem_cmp /Cop.sem_binarith /Cop.sem_cast /=. 
-  by case: (Archi.ptr64)=> //=.
+  move=> [] <- /= [] <- /=. by case: (Archi.ptr64)=> //=.
 + case: v2=> //=. case: t1=> //= p. case: p=> //=.
   case: t2=> //= p. case: p=> //= sz s sz' s' i i'. 
   case: s'=> //=.
@@ -645,20 +672,20 @@ move=> v1 v2 t1 t2 v cenv m /= ha. case: v1 ha=> //=.
     rewrite /Cop.sem_cmp /= /Cop.sem_binarith /= /Cop.sem_cast /=.
     case: ifP=> //= hi.
     + case: ifP=> //= hi'.
-      + case: Archi.ptr64=>//=.
+      + move=> [] <- /= [] <- /=. case: Archi.ptr64=>//=.
         + rewrite /Values.Val.of_bool /bool_to_int /=. by case: ifP=> //=.
         case: (intsize_eq Ctypes.I32 Ctypes.I32)=> //= heq.
         rewrite /Values.Val.of_bool /bool_to_int /=. by case: ifP=> //=.
-      case: Archi.ptr64=>//=.
+      move=> [] <- /= [] <- /=. case: Archi.ptr64=>//=.
       + rewrite /Values.Val.of_bool /bool_to_int /=. by case: ifP=> //=.
       case: (intsize_eq Ctypes.I32 Ctypes.I32)=> //= heq.
       rewrite /Values.Val.of_bool /bool_to_int /=. by case: ifP=> //=.
       case: ifP=> //= hi1.
-      + case: Archi.ptr64=>//=.
+      + move=> [] <- /= [] <- /=. case: Archi.ptr64=>//=.
         + rewrite /Values.Val.of_bool /bool_to_int /=. by case: ifP=> //=.
         case: (intsize_eq Ctypes.I32 Ctypes.I32)=> //= heq.
         rewrite /Values.Val.of_bool /bool_to_int /=. by case: ifP=> //=.
-      case: Archi.ptr64=>//=.
+      move=> [] <- /= [] <- /=. case: Archi.ptr64=>//=.
       + rewrite /Values.Val.of_bool /bool_to_int /=. by case: ifP=> //=.
       case: (intsize_eq Ctypes.I32 Ctypes.I32)=> //= heq.
       rewrite /Values.Val.of_bool /bool_to_int /=. by case: ifP=> //=.
@@ -666,20 +693,20 @@ move=> v1 v2 t1 t2 v cenv m /= ha. case: v1 ha=> //=.
    rewrite /Cop.sem_cmp /= /Cop.sem_binarith /= /Cop.sem_cast /=.
     case: ifP=> //= hi.
     + case: ifP=> //= hi'.
-      + case: Archi.ptr64=>//=.
+      + move=> [] <- /= [] <- /=. case: Archi.ptr64=>//=.
         + rewrite /Values.Val.of_bool /bool_to_int /=. by case: ifP=> //=.
         case: (intsize_eq Ctypes.I32 Ctypes.I32)=> //= heq.
         rewrite /Values.Val.of_bool /bool_to_int /=. by case: ifP=> //=.
-      case: Archi.ptr64=>//=.
+      move=> [] <- /= [] <- /=. case: Archi.ptr64=>//=.
       + rewrite /Values.Val.of_bool /bool_to_int /=. by case: ifP=> //=.
       case: (intsize_eq Ctypes.I32 Ctypes.I32)=> //= heq.
       rewrite /Values.Val.of_bool /bool_to_int /=. by case: ifP=> //=.
       case: ifP=> //= hi1.
-      + case: Archi.ptr64=>//=.
+      + move=> [] <- /= [] <- /=. case: Archi.ptr64=>//=.
         + rewrite /Values.Val.of_bool /bool_to_int /=. by case: ifP=> //=.
         case: (intsize_eq Ctypes.I32 Ctypes.I32)=> //= heq.
         rewrite /Values.Val.of_bool /bool_to_int /=. by case: ifP=> //=.
-      case: Archi.ptr64=>//=.
+      move=> [] <- /= [] <- /=. case: Archi.ptr64=>//=.
       + rewrite /Values.Val.of_bool /bool_to_int /=. by case: ifP=> //=.
       case: (intsize_eq Ctypes.I32 Ctypes.I32)=> //= heq.
       rewrite /Values.Val.of_bool /bool_to_int /=. by case: ifP=> //=.
@@ -690,17 +717,19 @@ case: p''=> //= sz s. case: t2=> //= b' b''. case: b''=> //= p1.
 by case: p1=> //=.
 Qed.
 
-Lemma transl_gt_cgt: forall v1 v2 t1 t2 v cenv m,
+Lemma transl_gt_cgt: forall v1 v2 t1 t2 v cenv m ct1 ct2,
 sem_binary_operation Gt v1 v2 t1 t2 = Some v -> 
-Cop.sem_binary_operation cenv (transBeePL_bop_bop Gt) (transBeePL_value_cvalue v1) 
-     (transBeePL_type t1) (transBeePL_value_cvalue v2) (transBeePL_type t2) m = 
+transBeePL_type t1 = OK ct1 ->
+transBeePL_type t2 = OK ct2 -> 
+Cop.sem_binary_operation cenv 
+  (transBeePL_bop_bop Gt) (transBeePL_value_cvalue v1) ct1 (transBeePL_value_cvalue v2) ct2 m = 
 Some (transBeePL_value_cvalue v). 
 Proof.
-move=> v1 v2 t1 t2 v cenv m /= ha. case: v1 ha=> //=.
+move=> v1 v2 t1 t2 v cenv m ct1 ct2 /= ha. case: v1 ha=> //=.
 + case: v2=> //=. case: t1=> //= p. case: p=> //=.
   case: t2=> //= p. case: p=> //= [] [] hv; subst; rewrite /=.
   rewrite /Cop.sem_cmp /Cop.sem_binarith /Cop.sem_cast /=. 
-  by case: (Archi.ptr64)=> //=.
+  move=> [] <- /= [] <- /=. by case: (Archi.ptr64)=> //=.
 + case: v2=> //=. case: t1=> //= p. case: p=> //=.
   case: t2=> //= p. case: p=> //= sz s sz' s' i i'. 
   case: s'=> //=.
@@ -708,20 +737,20 @@ move=> v1 v2 t1 t2 v cenv m /= ha. case: v1 ha=> //=.
     rewrite /Cop.sem_cmp /= /Cop.sem_binarith /= /Cop.sem_cast /=.
     case: ifP=> //= hi.
     + case: ifP=> //= hi'.
-      + case: Archi.ptr64=>//=.
+      + move=> [] <- /= [] <- /=. case: Archi.ptr64=>//=.
         + rewrite /Values.Val.of_bool /bool_to_int /=. by case: ifP=> //=.
         case: (intsize_eq Ctypes.I32 Ctypes.I32)=> //= heq.
         rewrite /Values.Val.of_bool /bool_to_int /=. by case: ifP=> //=.
-      case: Archi.ptr64=>//=.
+      move=> [] <- /= [] <- /=. case: Archi.ptr64=>//=.
       + rewrite /Values.Val.of_bool /bool_to_int /=. by case: ifP=> //=.
       case: (intsize_eq Ctypes.I32 Ctypes.I32)=> //= heq.
       rewrite /Values.Val.of_bool /bool_to_int /=. by case: ifP=> //=.
       case: ifP=> //= hi1.
-      + case: Archi.ptr64=>//=.
+      + move=> [] <- /= [] <- /=. case: Archi.ptr64=>//=.
         + rewrite /Values.Val.of_bool /bool_to_int /=. by case: ifP=> //=.
         case: (intsize_eq Ctypes.I32 Ctypes.I32)=> //= heq.
         rewrite /Values.Val.of_bool /bool_to_int /=. by case: ifP=> //=.
-      case: Archi.ptr64=>//=.
+      move=> [] <- /= [] <- /=. case: Archi.ptr64=>//=.
       + rewrite /Values.Val.of_bool /bool_to_int /=. by case: ifP=> //=.
       case: (intsize_eq Ctypes.I32 Ctypes.I32)=> //= heq.
       rewrite /Values.Val.of_bool /bool_to_int /=. by case: ifP=> //=.
@@ -729,20 +758,20 @@ move=> v1 v2 t1 t2 v cenv m /= ha. case: v1 ha=> //=.
    rewrite /Cop.sem_cmp /= /Cop.sem_binarith /= /Cop.sem_cast /=.
     case: ifP=> //= hi.
     + case: ifP=> //= hi'.
-      + case: Archi.ptr64=>//=.
+      + move=> [] <- /= [] <- /=. case: Archi.ptr64=>//=.
         + rewrite /Values.Val.of_bool /bool_to_int /=. by case: ifP=> //=.
         case: (intsize_eq Ctypes.I32 Ctypes.I32)=> //= heq.
         rewrite /Values.Val.of_bool /bool_to_int /=. by case: ifP=> //=.
-      case: Archi.ptr64=>//=.
+      move=> [] <- /= [] <- /=. case: Archi.ptr64=>//=.
       + rewrite /Values.Val.of_bool /bool_to_int /=. by case: ifP=> //=.
       case: (intsize_eq Ctypes.I32 Ctypes.I32)=> //= heq.
       rewrite /Values.Val.of_bool /bool_to_int /=. by case: ifP=> //=.
       case: ifP=> //= hi1.
-      + case: Archi.ptr64=>//=.
+      + move=> [] <- /= [] <- /=. case: Archi.ptr64=>//=.
         + rewrite /Values.Val.of_bool /bool_to_int /=. by case: ifP=> //=.
         case: (intsize_eq Ctypes.I32 Ctypes.I32)=> //= heq.
         rewrite /Values.Val.of_bool /bool_to_int /=. by case: ifP=> //=.
-      case: Archi.ptr64=>//=.
+      move=> [] <- /= [] <- /=. case: Archi.ptr64=>//=.
       + rewrite /Values.Val.of_bool /bool_to_int /=. by case: ifP=> //=.
       case: (intsize_eq Ctypes.I32 Ctypes.I32)=> //= heq.
       rewrite /Values.Val.of_bool /bool_to_int /=. by case: ifP=> //=.
@@ -753,17 +782,19 @@ case: p''=> //= sz s. case: t2=> //= b' b''. case: b''=> //= p1.
 by case: p1=> //=.
 Qed.
 
-Lemma transl_lte_cle: forall v1 v2 t1 t2 v cenv m,
+Lemma transl_lte_cle: forall v1 v2 t1 t2 v cenv m ct1 ct2,
 sem_binary_operation Lte v1 v2 t1 t2 = Some v -> 
-Cop.sem_binary_operation cenv (transBeePL_bop_bop Lte) (transBeePL_value_cvalue v1) 
-     (transBeePL_type t1) (transBeePL_value_cvalue v2) (transBeePL_type t2) m = 
+transBeePL_type t1 = OK ct1 ->
+transBeePL_type t2 = OK ct2 -> 
+Cop.sem_binary_operation cenv 
+(transBeePL_bop_bop Lte) (transBeePL_value_cvalue v1) ct1 (transBeePL_value_cvalue v2) ct2 m = 
 Some (transBeePL_value_cvalue v). 
 Proof.
-move=> v1 v2 t1 t2 v cenv m /= ha. case: v1 ha=> //=.
+move=> v1 v2 t1 t2 v cenv m ct1 ct2 /= ha. case: v1 ha=> //=.
 + case: v2=> //=. case: t1=> //= p. case: p=> //=.
   case: t2=> //= p. case: p=> //= [] [] hv; subst; rewrite /=.
   rewrite /Cop.sem_cmp /Cop.sem_binarith /Cop.sem_cast /=. 
-  by case: (Archi.ptr64)=> //=.
+  move=> [] <- /= [] <- /=. by case: (Archi.ptr64)=> //=.
 + case: v2=> //=. case: t1=> //= p. case: p=> //=.
   case: t2=> //= p. case: p=> //= sz s sz' s' i i'. 
   case: s'=> //=.
@@ -771,20 +802,20 @@ move=> v1 v2 t1 t2 v cenv m /= ha. case: v1 ha=> //=.
     rewrite /Cop.sem_cmp /= /Cop.sem_binarith /= /Cop.sem_cast /=.
     case: ifP=> //= hi.
     + case: ifP=> //= hi'.
-      + case: Archi.ptr64=>//=.
+      + move=> [] <- /= [] <- /=. case: Archi.ptr64=>//=.
         + rewrite /Values.Val.of_bool /bool_to_int /=. by case: ifP=> //=.
         case: (intsize_eq Ctypes.I32 Ctypes.I32)=> //= heq.
         rewrite /Values.Val.of_bool /bool_to_int /=. by case: ifP=> //=.
-      case: Archi.ptr64=>//=.
+      move=> [] <- /= [] <- /=. case: Archi.ptr64=>//=.
       + rewrite /Values.Val.of_bool /bool_to_int /=. by case: ifP=> //=.
       case: (intsize_eq Ctypes.I32 Ctypes.I32)=> //= heq.
       rewrite /Values.Val.of_bool /bool_to_int /=. by case: ifP=> //=.
       case: ifP=> //= hi1.
-      + case: Archi.ptr64=>//=.
+      + move=> [] <- /= [] <- /=. case: Archi.ptr64=>//=.
         + rewrite /Values.Val.of_bool /bool_to_int /=. by case: ifP=> //=.
         case: (intsize_eq Ctypes.I32 Ctypes.I32)=> //= heq.
         rewrite /Values.Val.of_bool /bool_to_int /=. by case: ifP=> //=.
-      case: Archi.ptr64=>//=.
+      move=> [] <- /= [] <- /=. case: Archi.ptr64=>//=.
       + rewrite /Values.Val.of_bool /bool_to_int /=. by case: ifP=> //=.
       case: (intsize_eq Ctypes.I32 Ctypes.I32)=> //= heq.
       rewrite /Values.Val.of_bool /bool_to_int /=. by case: ifP=> //=.
@@ -792,25 +823,25 @@ move=> v1 v2 t1 t2 v cenv m /= ha. case: v1 ha=> //=.
    rewrite /Cop.sem_cmp /= /Cop.sem_binarith /= /Cop.sem_cast /=.
     case: ifP=> //= hi.
     + case: ifP=> //= hi'.
-      + case: Archi.ptr64=>//=.
+      + move=> [] <- /= [] <- /=. case: Archi.ptr64=>//=.
         + rewrite /Values.Val.of_bool /bool_to_int /=. by case: ifP=> //=.
         case: (intsize_eq Ctypes.I32 Ctypes.I32)=> //= heq.
         rewrite /Values.Val.of_bool /bool_to_int /=. by case: ifP=> //=.
-      case: Archi.ptr64=>//=.
+      move=> [] <- /= [] <- /=. case: Archi.ptr64=>//=.
       + rewrite /Values.Val.of_bool /bool_to_int /=. by case: ifP=> //=.
       case: (intsize_eq Ctypes.I32 Ctypes.I32)=> //= heq.
       rewrite /Values.Val.of_bool /bool_to_int /=. by case: ifP=> //=.
       case: ifP=> //= hi1.
-      + case: Archi.ptr64=>//=.
+      + move=> [] <- /= [] <- /=. case: Archi.ptr64=>//=.
         + rewrite /Values.Val.of_bool /bool_to_int /=. by case: ifP=> //=.
         case: (intsize_eq Ctypes.I32 Ctypes.I32)=> //= heq.
         rewrite /Values.Val.of_bool /bool_to_int /=. by case: ifP=> //=.
-      case: Archi.ptr64=>//=.
+      move=> [] <- /= [] <- /=. case: Archi.ptr64=>//=.
       + rewrite /Values.Val.of_bool /bool_to_int /=. by case: ifP=> //=.
       case: (intsize_eq Ctypes.I32 Ctypes.I32)=> //= heq.
       rewrite /Values.Val.of_bool /bool_to_int /=. by case: ifP=> //=.
  + case: v2=> //=. case: t1=> //= p. case: p=> //=. case: t2=> //= p.
-   case: p=> //= b b'. case: ifP=> //= hb [] hv; subst.
+   case: p=> //= b b'. case: ifP=> //= hb [] hv; subst. move=> [] <- /= [] <- /=. 
    rewrite /Cop.sem_cmp /= /Cop.sem_binarith /Cop.sem_cast /Cop.classify_cast /=.
    case: ifP=> //=.
    + case: ifP=> //=. 
@@ -838,16 +869,18 @@ by case: p1=> //=.
 Qed.
 
 
-Lemma transl_gte_cge: forall v1 v2 t1 t2 v cenv m,
+Lemma transl_gte_cge: forall v1 v2 t1 t2 v cenv m ct1 ct2,
 sem_binary_operation Gte v1 v2 t1 t2 = Some v -> 
-Cop.sem_binary_operation cenv (transBeePL_bop_bop Gte) (transBeePL_value_cvalue v1) 
-     (transBeePL_type t1) (transBeePL_value_cvalue v2) (transBeePL_type t2) m = 
+transBeePL_type t1 = OK ct1 ->
+transBeePL_type t2 = OK ct2 -> 
+Cop.sem_binary_operation cenv 
+  (transBeePL_bop_bop Gte) (transBeePL_value_cvalue v1) ct1 (transBeePL_value_cvalue v2) ct2 m = 
 Some (transBeePL_value_cvalue v). 
-move=> v1 v2 t1 t2 v cenv m /= ha. case: v1 ha=> //=.
+move=> v1 v2 t1 t2 v cenv m ct1 ct2 /= ha. case: v1 ha=> //=.
 + case: v2=> //=. case: t1=> //= p. case: p=> //=.
   case: t2=> //= p. case: p=> //= [] [] hv; subst; rewrite /=.
   rewrite /Cop.sem_cmp /Cop.sem_binarith /Cop.sem_cast /=. 
-  by case: (Archi.ptr64)=> //=.
+  move=> [] <- /= [] <- /=. by case: (Archi.ptr64)=> //=.
 + case: v2=> //=. case: t1=> //= p. case: p=> //=.
   case: t2=> //= p. case: p=> //= sz s sz' s' i i'. 
   case: s'=> //=.
@@ -855,20 +888,20 @@ move=> v1 v2 t1 t2 v cenv m /= ha. case: v1 ha=> //=.
     rewrite /Cop.sem_cmp /= /Cop.sem_binarith /= /Cop.sem_cast /=.
     case: ifP=> //= hi.
     + case: ifP=> //= hi'.
-      + case: Archi.ptr64=>//=.
+      + move=> [] <- /= [] <- /=. case: Archi.ptr64=>//=.
         + rewrite /Values.Val.of_bool /bool_to_int /=. by case: ifP=> //=.
         case: (intsize_eq Ctypes.I32 Ctypes.I32)=> //= heq.
         rewrite /Values.Val.of_bool /bool_to_int /=. by case: ifP=> //=.
-      case: Archi.ptr64=>//=.
+      move=> [] <- /= [] <- /=. case: Archi.ptr64=>//=.
       + rewrite /Values.Val.of_bool /bool_to_int /=. by case: ifP=> //=.
       case: (intsize_eq Ctypes.I32 Ctypes.I32)=> //= heq.
       rewrite /Values.Val.of_bool /bool_to_int /=. by case: ifP=> //=.
       case: ifP=> //= hi1.
-      + case: Archi.ptr64=>//=.
+      + move=> [] <- /= [] <- /=. case: Archi.ptr64=>//=.
         + rewrite /Values.Val.of_bool /bool_to_int /=. by case: ifP=> //=.
         case: (intsize_eq Ctypes.I32 Ctypes.I32)=> //= heq.
         rewrite /Values.Val.of_bool /bool_to_int /=. by case: ifP=> //=.
-      case: Archi.ptr64=>//=.
+      move=> [] <- /= [] <- /=. case: Archi.ptr64=>//=.
       + rewrite /Values.Val.of_bool /bool_to_int /=. by case: ifP=> //=.
       case: (intsize_eq Ctypes.I32 Ctypes.I32)=> //= heq.
       rewrite /Values.Val.of_bool /bool_to_int /=. by case: ifP=> //=.
@@ -876,27 +909,27 @@ move=> v1 v2 t1 t2 v cenv m /= ha. case: v1 ha=> //=.
    rewrite /Cop.sem_cmp /= /Cop.sem_binarith /= /Cop.sem_cast /=.
     case: ifP=> //= hi.
     + case: ifP=> //= hi'.
-      + case: Archi.ptr64=>//=.
+      + move=> [] <- /= [] <- /=. case: Archi.ptr64=>//=.
         + rewrite /Values.Val.of_bool /bool_to_int /=. by case: ifP=> //=.
         case: (intsize_eq Ctypes.I32 Ctypes.I32)=> //= heq.
         rewrite /Values.Val.of_bool /bool_to_int /=. by case: ifP=> //=.
-      case: Archi.ptr64=>//=.
+      move=> [] <- /= [] <- /=. case: Archi.ptr64=>//=.
       + rewrite /Values.Val.of_bool /bool_to_int /=. by case: ifP=> //=.
       case: (intsize_eq Ctypes.I32 Ctypes.I32)=> //= heq.
       rewrite /Values.Val.of_bool /bool_to_int /=. by case: ifP=> //=.
       case: ifP=> //= hi1.
-      + case: Archi.ptr64=>//=.
+      + move=> [] <- /= [] <- /=. case: Archi.ptr64=>//=.
         + rewrite /Values.Val.of_bool /bool_to_int /=. by case: ifP=> //=.
         case: (intsize_eq Ctypes.I32 Ctypes.I32)=> //= heq.
         rewrite /Values.Val.of_bool /bool_to_int /=. by case: ifP=> //=.
-      case: Archi.ptr64=>//=.
+      move=> [] <- /= [] <- /=. case: Archi.ptr64=>//=.
       + rewrite /Values.Val.of_bool /bool_to_int /=. by case: ifP=> //=.
       case: (intsize_eq Ctypes.I32 Ctypes.I32)=> //= heq.
       rewrite /Values.Val.of_bool /bool_to_int /=. by case: ifP=> //=.
  + case: v2=> //=. case: t1=> //= p. case: p=> //=. case: t2=> //= p.
    case: p=> //= b b'. case: ifP=> //= hb [] hv; subst.
    rewrite /Cop.sem_cmp /= /Cop.sem_binarith /Cop.sem_cast /Cop.classify_cast /=.
-   case: ifP=> //=.
+   move=> [] <- /= [] <- /=. case: ifP=> //=.
    + case: ifP=> //=. 
      + case: Archi.ptr64=> //=.
        + rewrite /Values.Val.of_bool /bool_to_int /=. case: b hb=> //=.
@@ -921,42 +954,44 @@ case: p''=> //= sz s. case: t2=> //= b' b''. case: b''=> //= p1.
 by case: p1=> //=.
 Qed.
 
-Lemma transl_bop_cbop : forall cenv op v1 v2 t1 t2 v m,
-sem_binary_operation op v1 v2 t1 t2 = Some v -> 
-Cop.sem_binary_operation cenv (transBeePL_bop_bop op) (transBeePL_value_cvalue v1) 
-   (transBeePL_type t1) (transBeePL_value_cvalue v2) (transBeePL_type t2) m = Some (transBeePL_value_cvalue v).
+Lemma transl_bop_cbop : forall cenv op v1 v2 t1 t2 v ct1 ct2 m,
+sem_binary_operation op v1 v2 t1 t2 = Some v ->
+transBeePL_type t1 = OK ct1 ->
+transBeePL_type t2 = OK ct2 -> 
+Cop.sem_binary_operation cenv 
+(transBeePL_bop_bop op) (transBeePL_value_cvalue v1) ct1 (transBeePL_value_cvalue v2) ct2 m = Some (transBeePL_value_cvalue v).
 Proof.
 intros. destruct op; simpl; auto; subst.
 (* Add *)
-+ by have := (transl_plus_cadd v1 v2 t1 t2 v cenv m H).
++ by have := (transl_plus_cadd v1 v2 t1 t2 v cenv m ct1 ct2 H H0 H1).
 (* Sub *)
-+ by have := (transl_minus_csub v1 v2 t1 t2 v cenv m H).
++ by have := (transl_minus_csub v1 v2 t1 t2 v cenv m ct1 ct2 H H0 H1).
 (* Mult *)
-+ by have := (transl_mult_cmul v1 v2 t1 t2 v cenv m H).
++ by have := (transl_mult_cmul v1 v2 t1 t2 v cenv m ct1 ct2 H H0 H1).
 (* Div *)
-+ by have := (transl_div_cdiv v1 v2 t1 t2 v cenv m H).
++ by have := (transl_div_cdiv v1 v2 t1 t2 v cenv m ct1 ct2 H H0 H1).
 (* And *)
-+ by have := (transl_and_cand v1 v2 t1 t2 v cenv m H).
++ by have := (transl_and_cand v1 v2 t1 t2 v cenv m ct1 ct2 H H0 H1).
 (* Or *)
-+ by have := (transl_or_cor v1 v2 t1 t2 v cenv m H).
++ by have := (transl_or_cor v1 v2 t1 t2 v cenv m ct1 ct2 H H0 H1).
 (* Xor *)
-+ by have := (transl_xor_cxor v1 v2 t1 t2 v cenv m H).
++ by have := (transl_xor_cxor v1 v2 t1 t2 v cenv m ct1 ct2 H H0 H1).
 (* Shl *)
-+ by have := (transl_shl_cshl v1 v2 t1 t2 v cenv m H).
++ by have := (transl_shl_cshl v1 v2 t1 t2 v cenv m ct1 ct2 H H0 H1).
 (* Shr *)
-+ by have := (transl_shr_cshr v1 v2 t1 t2 v cenv m H).
++ by have := (transl_shr_cshr v1 v2 t1 t2 v cenv m ct1 ct2 H H0 H1).
 (* Eq *)
-+ by have := (transl_eq_ceq v1 v2 t1 t2 v cenv m H).
++ by have := (transl_eq_ceq v1 v2 t1 t2 v cenv m ct1 ct2 H H0 H1).
 (* Ne *)
-+ by have := (transl_neq_cneq v1 v2 t1 t2 v cenv m H).
++ by have := (transl_neq_cneq v1 v2 t1 t2 v cenv m ct1 ct2 H H0 H1).
 (* Lt *)
-+ by have := (transl_lt_clt v1 v2 t1 t2 v cenv m H).
++ by have := (transl_lt_clt v1 v2 t1 t2 v cenv m ct1 ct2 H H0 H1).
 (* Le *)
-+ by have := (transl_lte_cle v1 v2 t1 t2 v cenv m H).
++ by have := (transl_lte_cle v1 v2 t1 t2 v cenv m ct1 ct2 H H0 H1).
 (* Gt *)
-+ by have := (transl_gt_cgt v1 v2 t1 t2 v cenv m H).
++ by have := (transl_gt_cgt v1 v2 t1 t2 v cenv m ct1 ct2 H H0 H1).
 (* Ge *)
-by have := (transl_gte_cge v1 v2 t1 t2 v cenv m H).
+by have := (transl_gte_cge v1 v2 t1 t2 v cenv m ct1 ct2 H H0 H1).
 Qed.
 
 
